
\documentclass[twocolumn]{ctexart}
% \documentclass[onecolumn]{ctexart}

\usepackage{geometry}
\geometry{a4paper,left=1cm,right=1cm,top=1.4cm,bottom=1cm}

\usepackage{amsmath,amssymb,amsfonts}
\usepackage{xcolor}
\usepackage{graphicx}  % for \resizebox
\usepackage{arydshln}



\usepackage{hyperref}
\hypersetup{
    pdfstartview={XYZ null null 1.25},  % XYZ <left> <top> <zoom> : Sets a coordinate and a zoom factor. If anyone is null, the source link value is used.
    % pdfstartview={FitH  null},           % FitH <top> : fit the width of the page to the window
    pdfpagelayout=OneColumn,  % SinglePage/OneColumn/...
    % 
    bookmarks=true,
    bookmarksnumbered=true,
    bookmarksopen=true,  % whether bookmark tree is expanded when opening pdf
    pdfpagemode=UseOutlines,  % UseOutlines: show bookmarks panel when opening pdf
    % 
    linkbordercolor=blue,
}



\begin{document}

\leftline{2023\_1019\_0148\_21}





% IIIIIIIIIIIIIIIIIIIIIIIIIIIIIIIIIIIIIIIIIIIIIIIIIIIIIIIIIIIIIIIIIIIIIIIIIIIIIIIIIIIIIIIIIIIIIIIIIIII
\vspace{30pt}
\section{Preliminaries}

% =================================================================
% \iffalse
\subsection{Standard Form of LP}

Any unbounded variable $x$ can be replaced by a pair of non-negative variables $(u,v)$.
\begin{equation}
    \begin{aligned}
        \label{eq:var_unbounded_to_nonnegative}
        \begin{cases}
            x = u - v \\
            u \geq 0  \\
            v \geq 0  \\
        \end{cases}
    \end{aligned}
\end{equation}

Any in-equality constraint can be converted into an equality constraint,
by introducing an additional assistant non-negative variable $x'$.
\begin{equation}
    \begin{aligned}
        \label{eq:cons_inequal_to_equal}
        \mathbf{a}_i^T  \mathbf{x}  \geq  b_i
        & \qquad \Leftrightarrow \qquad
        \begin{cases}
            \mathbf{a}_i^T \mathbf{x}  -  x'  &=  b_i \\
            x' &\geq 0 \\
        \end{cases}
        \\
        & \qquad \Leftrightarrow \qquad
        \begin{cases}
            \begin{bmatrix} \mathbf{a}_i^T &  (-1) \end{bmatrix}
            \begin{bmatrix} \mathbf{x}     \\ x' \end{bmatrix}
            &= b_i
            \\
            x' &\geq 0 \\
        \end{cases}
    \end{aligned}
\end{equation}

So we can safely represent any Linear Programming (LP) problem in its standard form,
with only non-negative variables and only equality constraints.
% \fi





% \subsection{What about LPs in standard form}
% ----------------------------
\subsubsection{Example}
% \subsubsection{Example 1:}

The LP with equalities and in-equalities
\begin{equation}
    \begin{aligned}
        \label{eq:mixed_equal_and_inequal}
        \text{Minimize} \qquad &
            \mathbf{c}^T  \mathbf{\color{red} x}
        \\
        \text{s.t.} \qquad &
            \begin{cases}
                \mathbf{A}^{(e)}  \mathbf{\color{red} x}  &  =     \mathbf{b}^{(e)}  {\color{gray} \quad \in \mathbb{R}^{m^{(e)} \times 1}}  \\
                \mathbf{A}^{(i)}  \mathbf{\color{red} x}  &  \geq  \mathbf{b}^{(i)}  {\color{gray} \quad \in \mathbb{R}^{m^{(i)} \times 1}}  \\
                                  \mathbf{\color{red} x}  &  \geq  \mathbf{0}        {\color{gray} \quad \in \mathbb{R}^{n \times 1}}  \\
            \end{cases}
    \end{aligned}
\end{equation}
% can be transformed to elininate in-equalities
can be transformed to a standard form without in-equalities
\begin{equation}
    \begin{aligned}
        \label{eq:only_equal}
        \text{Minimize} \qquad &
            \mathbf{c}^T  \mathbf{\color{red} x}
        \\
        \text{s.t.} \qquad &
            \begin{cases}
                \mathbf{A}^{(e)}  \mathbf{\color{red} x}                 &  =     \mathbf{b}^{(e)}  {\color{gray} \quad \in \mathbb{R}^{m^{(e)} \times 1}}  \\
                \mathbf{A}^{(i)}  \mathbf{\color{red} x}  -  \mathbf{y}  &  =     \mathbf{b}^{(i)}  {\color{gray} \quad \in \mathbb{R}^{m^{(i)} \times 1}}  \\
                                  \mathbf{\color{red} x}                 &  \geq  \mathbf{0}        {\color{gray} \quad \in \mathbb{R}^{n       \times 1}}  \\
                                  \mathbf{\color{red} y}                 &  \geq  \mathbf{0}        {\color{gray} \quad \in \mathbb{R}^{m^{(i)} \times 1}}  \\
            \end{cases}
    \end{aligned}
\end{equation}




% =================================================================
% \iffalse
\subsection{In-equality Form of LP}

Conversely,
any equality constraint can also be converted into in-equality constraints,
by using a pair of "opposite" constraints.

\begin{equation}
    \begin{aligned}
        \label{eq:cons_equal_to_inequal}
        \mathbf{a}_i^T  \mathbf{x}  =  b_i
        & \qquad \Leftrightarrow \qquad
        \begin{cases}
            \mathbf{a}_i^T \mathbf{x}  \geq  b_i \\
            \mathbf{a}_i^T \mathbf{x}  \leq  b_i \\
        \end{cases}
        \\
        & \qquad \Leftrightarrow \qquad
        \begin{cases}
            +\mathbf{a}_i^T \mathbf{x}  \geq  +b_i \\
            -\mathbf{a}_i^T \mathbf{x}  \geq  -b_i \\
        \end{cases}
        \\
        & \qquad \Leftrightarrow \qquad
        \begin{cases}
            \begin{bmatrix}  \mathbf{a}_i^T  \\  -\mathbf{a}_i^T  \end{bmatrix}
            \mathbf{x}
            &\geq
            \begin{bmatrix}  +b_i  \\  -b_i  \end{bmatrix}
        \end{cases}
    \end{aligned}
\end{equation}



% ----------------------------
\subsubsection{Example}

The LP with equalities and in-equalities Eq.(\ref{eq:mixed_equal_and_inequal})
can also be transformed to an in-equality form without equalities
\begin{equation}
    \begin{aligned}
        \label{eq:only_inequal}
        \text{Minimize} \qquad &
            \mathbf{c}^T  \mathbf{\color{red} x}
        \\
        \text{s.t.} \qquad &
            \begin{cases}
                +\mathbf{A}^{(e)}  \mathbf{\color{red} x}  &  \geq  +\mathbf{b}^{(e)}  {\color{gray} \quad \in \mathbb{R}^{m^{(e)} \times 1}}  \\
                -\mathbf{A}^{(e)}  \mathbf{\color{red} x}  &  \geq  -\mathbf{b}^{(e)}  {\color{gray} \quad \in \mathbb{R}^{m^{(e)} \times 1}}  \\
                 \mathbf{A}^{(i)}  \mathbf{\color{red} x}  &  \geq   \mathbf{b}^{(i)}  {\color{gray} \quad \in \mathbb{R}^{m^{(i)} \times 1}}  \\
                                   \mathbf{\color{red} x}  &  \geq   \mathbf{0}        {\color{gray} \quad \in \mathbb{R}^{n       \times 1}}  \\
            \end{cases}
    \end{aligned}
\end{equation}










% IIIIIIIIIIIIIIIIIIIIIIIIIIIIIIIIIIIIIIIIIIIIIIIIIIIIIIIIIIIIIIIIIIIIIIIIIIIIIIIIIIIIIIIIIIIIIIIIIIII
\clearpage
\vspace{30pt}
\section{LP and Duality}

% =================================================================
\subsection{Definition of Dual}
\label{sec:def_of_dual}

Assume
$\mathbf{A} \in \mathbb{R}^{m \times n}$
,
$\mathbf{b} \in \mathbb{R}^{m \times 1}$
,
$\mathbf{c} \in \mathbb{R}^{n \times 1}$
.
% A LP problem
The LP problem \textbf{\color{blue} (in in-equality form)}
\begin{equation}
    \begin{aligned}
        \label{eq:primal}
        \text{Minimize} \qquad &
            \mathbf{c}^T  \mathbf{\color{red} x}
        \\
        \text{s.t.} \qquad &
            % &  A  \mathbf{x}  &  \geq  \mathbf{b}  \\
            % &     \mathbf{x}  &   \geq  \mathbf{0}  \\
            \begin{cases}
                \mathbf{A}  \mathbf{\color{red} x}  &  \geq  \mathbf{b}  {\color{gray} \quad \in \mathbb{R}^{m \times 1}}  \\
                            \mathbf{\color{red} x}  &  \geq  \mathbf{0}  {\color{gray} \quad \in \mathbb{R}^{n \times 1}}  \\
            \end{cases}
    \end{aligned}
\end{equation}
has a dual problem defined as
\begin{equation}
    \begin{aligned}
        \label{eq:dual}
        \text{Maximize} \qquad &
            \mathbf{b}^T  \mathbf{\color{red} \lambda}
        \\
        \text{s.t.} \qquad &
            \begin{cases}
                \mathbf{A}^T  \mathbf{\color{red} \lambda}  &  \leq  \mathbf{c}  {\color{gray} \quad \in \mathbb{R}^{n \times 1}}  \\
                              \mathbf{\color{red} \lambda}  &  \geq  \mathbf{0}  {\color{gray} \quad \in \mathbb{R}^{m \times 1}}  \\
            \end{cases}
    \end{aligned}
\end{equation}
% and note that,
and we can conclude that the dual derivation process is simple:
\begin{itemize}
    \item  ($\mathbf{A} \Leftrightarrow \mathbf{A}^T$) coefficient matrix is transposed
    \item  ($\mathbf{b} \Leftrightarrow \mathbf{c}$) cost and constraint vectors are interchanged
    \item  ($\leq \  \Leftrightarrow \  \geq$) constraint in-equalities are reversed
    \item  (maximizing $\Leftrightarrow$ minimizing) optimization direction is reversed
\end{itemize}
and also note that the sizes/lengths of matrices/vectors are changed accordingly.


\vspace{40pt}


Following this definition,
the LP problem \textbf{\color{blue} (in standard form)}
\begin{equation}
    \begin{aligned}
        \label{eq:primal_standard}
        \text{Minimize} \qquad &
            \mathbf{c}^T  \mathbf{\color{red} x}
        \\
        \text{s.t.} \qquad &
            \begin{cases}
                \mathbf{A}  \mathbf{\color{red} x}  &  =     \mathbf{b}  {\color{gray} \quad \in \mathbb{R}^{m \times 1}}  \\
                            \mathbf{\color{red} x}  &  \geq  \mathbf{0}  {\color{gray} \quad \in \mathbb{R}^{n \times 1}}  \\
            \end{cases}
    \end{aligned}
\end{equation}
which can be converted into in-equality form as
\begin{equation}
    \begin{aligned}
        \label{eq:primal_standard_converted}
        \text{Minimize} \qquad &
            \mathbf{c}^T  \mathbf{\color{red} x}
        \\
        \text{s.t.} \qquad &
            \begin{cases}
                % +\mathbf{A}  \mathbf{\color{red} x}  &  \geq  +\mathbf{b}  {\color{gray} \quad \in \mathbb{R}^{m \times 1}}  \\
                % -\mathbf{A}  \mathbf{\color{red} x}  &  \geq  -\mathbf{b}  {\color{gray} \quad \in \mathbb{R}^{m \times 1}}  \\
                \begin{bmatrix}  +\mathbf{A}  \\  -\mathbf{A} \end{bmatrix}
                \mathbf{\color{red} x}
                &  \geq
                \begin{bmatrix}  +\mathbf{b}  \\  -\mathbf{b} \end{bmatrix}
                {\color{gray} \quad \in \mathbb{R}^{(2m) \times 1}}  \\
                             \mathbf{\color{red} x}  &  \geq   \mathbf{0}  {\color{gray} \quad \in \mathbb{R}^{n \times 1}}  \\
            \end{cases}
    \end{aligned}
\end{equation}
should have a dual problem as
\begin{equation}
    \begin{aligned}
        \label{eq:primal_standard_dual}
        \text{Maximize} \qquad &
            \begin{bmatrix}  +\mathbf{b}^T  &  -\mathbf{b}^T \end{bmatrix}
            \mathbf{\color{red} \lambda}
        \\
        \text{s.t.} \qquad &
            \begin{cases}
                \begin{bmatrix}  +\mathbf{A}^T  &  -\mathbf{A}^T \end{bmatrix}
                \mathbf{\color{red} \lambda}  &  \leq  \mathbf{c}  {\color{gray} \quad \in \mathbb{R}^{n \times 1}}  \\
                \mathbf{\color{red} \lambda}  &  \geq  \mathbf{0}  {\color{gray} \quad \in \mathbb{R}^{(2m) \times 1}}  \\
            \end{cases}
    \end{aligned}
\end{equation}
Partitioning $\mathbf{\lambda} {\color{gray} \in \mathbb{R}^{(2m) \times 1}}$
as $\begin{bmatrix}  \mathbf{\lambda}_1  {\color{gray} \quad \in \mathbb{R}^{m \times 1}}  \\  \mathbf{\lambda}_2  {\color{gray} \quad \in \mathbb{R}^{m \times 1}} \end{bmatrix}$
and we have
\begin{equation}
    \begin{aligned}
        \label{eq:primal_standard_dual_partitioned}
        \text{Maximize} \qquad &
            % +\mathbf{b}^T
            % % \mathbf{\color{red} \lambda_1}
            % {\color{red} \mathbf{\lambda}_1}
            % -\mathbf{b}^T
            % % \mathbf{\color{red} \lambda_2}
            % {\color{red} \mathbf{\lambda}_2}
            % =
            \mathbf{b}^T
            % (\mathbf{\color{red} \lambda_1} - \mathbf{\color{red} \lambda_2})
            ({\color{red} \mathbf{\lambda}_1} - {\color{red} \mathbf{\lambda}_2})
        \\
        \text{s.t.} \qquad &
            \begin{cases}
                % +\mathbf{A}^T
                % % \mathbf{\color{red} \lambda_1}
                % {\color{red} \mathbf{\lambda}_1}
                % -\mathbf{A}^T
                % % \mathbf{\color{red} \lambda_2}
                % {\color{red} \mathbf{\lambda}_2}
                % =
                \mathbf{A}^T
                % (\mathbf{\color{red} \lambda_1} - \mathbf{\color{red} \lambda_2})
                ({\color{red} \mathbf{\lambda}_1} - {\color{red} \mathbf{\lambda}_2})
                &  \leq  \mathbf{c}  {\color{gray} \quad \in \mathbb{R}^{n \times 1}}
                \\
                {\color{red} \mathbf{\lambda}_1}  &  \geq  \mathbf{0}  {\color{gray} \quad \in \mathbb{R}^{(m) \times 1}}
                \\
                {\color{red} \mathbf{\lambda}_2}  &  \geq  \mathbf{0}  {\color{gray} \quad \in \mathbb{R}^{(m) \times 1}}
                \\
            \end{cases}
    \end{aligned}
\end{equation}
and we can safely combine the free non-negative variables pairs $\mathbf{\lambda}' = (\mathbf{\lambda}_1 - \mathbf{\lambda}_2)$, resulting in
\begin{equation}
    \begin{aligned}
        \label{eq:primal_standard_dual_partitioned_combined}
        \text{Maximize} \qquad &
            \mathbf{b}^T
            % \mathbf{\color{red} \lambda'}
            {\color{red} \mathbf{\lambda}'}
        \\
        \text{s.t.} \qquad &
            \begin{cases}
                \mathbf{A}^T
                {\color{red} \mathbf{\lambda}'}
                &  \leq  \mathbf{c}  {\color{gray} \quad \in \mathbb{R}^{n \times 1}}
                \\
                {\color{red} \mathbf{\lambda}'}  &  \geq  -\mathbf{\infty}  {\color{gray} \quad \in \mathbb{R}^{m \times 1}}
                \\
                & \text{\color{red}  (variables not necessarily non-negative)}
                \\
            \end{cases}
    \end{aligned}
\end{equation}





% =================================================================
\subsection{The Duality Theorem}

So what is the relationship between Eq.(\ref{eq:primal}) and its dual Eq.(\ref{eq:dual}) defined in section \ref{sec:def_of_dual} ?

We will explore
% based on the pair of dual
, based on the dual of standard form,
Eq.(\ref{eq:primal_standard}) and Eq.(\ref{eq:primal_standard_dual_partitioned_combined}).


% ----------------------------
\subsubsection{Weak Duality Lemma}

% If
% $\mathbf{x}$ is feasible in Eq.(\ref{eq:primal_standard})
% and
% $\mathbf{\lambda}'$ is feasible in Eq.(\ref{eq:primal_standard_dual_partitioned_combined}),

If
Eq.(\ref{eq:primal_standard})
and
Eq.(\ref{eq:primal_standard_dual_partitioned_combined})
are both feasible,
then
any feasible solution $\mathbf{x}$        for Eq.(\ref{eq:primal_standard})
as well as
any feasible solution $\mathbf{\lambda}'$ for Eq.(\ref{eq:primal_standard_dual_partitioned_combined})
satisfies:


\begin{equation}
    \begin{aligned}
        \label{eq:weak_duality_lemma}
        &
        \mathbf{b}^T
        {\color{red} \mathbf{\lambda}'}
        % =&
        % {\color{red} \mathbf{\lambda}'{}^T}
        % \mathbf{b}
        % \\=&
        % {\color{red} \mathbf{\lambda}'{}^T}
        % \mathbf{A}
        % {\color{red} \mathbf{x}}
        \\=&
        (
            \mathbf{A}
            {\color{red} \mathbf{x}}
        )^T
        {\color{red} \mathbf{\lambda}'}
        % \qquad \text{\color{gray} by constraints in Eq.(\ref{eq:primal_standard})}
        \qquad {\color{gray} \text{by} \quad
            \mathbf{A}  \mathbf{x}  =  \mathbf{b}  \quad \text{in Eq.(\ref{eq:primal_standard})}
        }
        \\=&
        {\color{red} \mathbf{x}^T}
        (
            \mathbf{A}^T
            {\color{red} \mathbf{\lambda}'}
        )
        \\ \leq &
        {\color{red} \mathbf{x}^T}
        \mathbf{c}
        % \qquad \text{\color{gray} by constraints in Eq.(\ref{eq:primal_standard_dual_partitioned_combined})}
        \qquad {\color{gray} \text{by} \quad
            \begin{cases}
                \mathbf{A}^T  \mathbf{\lambda}'  \leq  \mathbf{c}  \quad \text{in Eq.(\ref{eq:primal_standard_dual_partitioned_combined})}
                \\
                \mathbf{x} \geq \mathbf{0}                         \quad \text{in Eq.(\ref{eq:primal_standard})}
            \end{cases}
        }
        \\=&
        \mathbf{c}^T
        {\color{red} \mathbf{x}}
    \end{aligned}
\end{equation}
% meaning that the objectives of a pair of feasible solutions
meaning that,
\begin{itemize}
    \item
    the objective of \textbf{any feasible} solution of a standard form LP as Eq.(\ref{eq:primal_standard})
    should always be larger than or equal to
    the objective of \textbf{any feasible} solution of its dual as Eq.(\ref{eq:primal_standard_dual_partitioned_combined}).
\end{itemize}
and therefore,
\begin{itemize}
    \item
    If either problem has an unbounded optimal objective,
    the other problem will be in-feasible.
    \item
    If both Eq.(\ref{eq:primal_standard}) and Eq.(\ref{eq:primal_standard_dual_partitioned_combined}) are feasible,
    the objective of \textbf{the optimal} solution of a standard form LP as Eq.(\ref{eq:primal_standard})
    should always be larger than or equal to
    the objective of \textbf{the optimal} solution of its dual as Eq.(\ref{eq:primal_standard_dual_partitioned_combined}).
    % (Note that Eq.(\ref{eq:primal_standard}) seeks for minimum, and Eq.(\ref{eq:primal_standard_dual_partitioned_combined}) seeks for maximum.)
    \begin{itemize}
        \item
        If we come across a pair of feasible solutions $(\mathbf{x}, \mathbf{\lambda}')$ where the equality holds,
        then they should be (one of) the corresponding optimal solutions of each problem.
    \end{itemize}
\end{itemize}
(Note that Eq.(\ref{eq:primal_standard}) seeks for minimum, and Eq.(\ref{eq:primal_standard_dual_partitioned_combined}) seeks for maximum.)



% ----------------------------
\subsubsection{Strong Duality Theorem}

% But, whether we can achieve this equality?
% But, can we (always) achieve this equality in Eq.(\ref{eq:weak_duality_lemma})?
However,
the above comparison is weak, and
these questions currently remain:
\begin{itemize}
    \item
    If either problem is in-feasible,
    should the other problem have an unbounded optimal objective?
    \item
    If either problem has a finite optimal objective,
    should the other problem also have a finite optimal objective?
    \item
    If both Eq.(\ref{eq:primal_standard}) and Eq.(\ref{eq:primal_standard_dual_partitioned_combined}) are feasible,
    % can we (always?) achieve that equality in Eq.(\ref{eq:weak_duality_lemma}),
    % e.g.,
    % can the two problems (always?) have the same optimal objective?
    in which case the two problems have the equal optimal objective?
\end{itemize}

TODO


\begin{equation}
    \begin{aligned}
        % \label{eq:}
    \end{aligned}
\end{equation}




\begin{equation}
    \begin{aligned}
        % \label{eq:}
    \end{aligned}
\end{equation}






\end{document}

